

Minor Exam (20%)

● Graded

Student

Kushagra Gupta

Total Points

41 / 50 pts

Question 1

Q1 (a)

5 / 5 pts

✓ + 1 pt $\text{atn}(p) = 1$

✓ + 1 pt $\text{atn}(\perp) = 0$

✓ + 1 pt $\text{atn}(\neg\alpha) = \text{atn}(\alpha)$

✓ + 1 pt $\text{atn}(\alpha \circ \beta) = |\text{atoms}(\alpha) \cup \text{atoms}(\beta)|$ or $\text{atn}(\alpha) + \text{atn}(\beta) - |\text{atoms}(\alpha) \cap \text{atoms}(\beta)|$ $\circ \in \{\wedge, \vee, \supset\}$

✓ + 1 pt Definition of atoms (inductive or $\text{sf}(\alpha) \cap AP$)

+ 0 pts Incorrect/Not attempted

Question 2

Q1 (b)

5 / 5 pts

✓ + 0.5 pts $\text{qd}(t_1 \equiv t_2) = 0$

✓ + 0.5 pts $\text{qd}(P(t_1, \dots, t_n)) = 0$

✓ + 1 pt $\text{qd}(\neg\alpha) = \text{qd}(\alpha)$

✓ + 1 pt $\text{qd}(\alpha \circ \beta) = \max(\text{qd}(\alpha), \text{qd}(\beta))$ $\circ \in \{\wedge, \vee, \supset\}$

✓ + 1 pt $\text{qd}(\exists x. [\alpha]) = 1 + \text{qd}(\alpha)$

✓ + 1 pt $\text{qd}(\forall x. [\alpha]) = 1 + \text{qd}(\alpha)$

+ 0 pts Incorrect/Not Attempt

Question 3

Q2 (a)



Resolved 3 / 4 pts

+ 4 pts Correct

+ 0 pts Incorrect

✓ + 1 pt Disjunction to figure out the leftmost point j where the first flip from 0 to 1 occurs✓ + 1 pt Conjunction to say that the c and d values are the same from 1 through $j - 1$ ✓ + 1 pt Conjunction to say that after j , if there are any positions, c might have been 1, but got flipped to 0 in d

+ 1 pt Something of the form $\bigvee_{1 \leq j \leq n} [(\neg c_j \wedge d_j) \wedge \bigwedge_{1 \leq i \leq j-1} ((c_i \wedge d_i) \vee (\neg c_i \wedge \neg d_i)) \wedge \bigwedge_{j+1 \leq i \leq n} ((c_i \wedge \neg d_i))]$

🗨 Unclear answer

🔄 Regrade Request

Submitted on: Oct 01

Dear sir/ma'am,

Could you please review my answer and consider the following request? I mentioned the exact same expression as the rubric -

$\bigvee_{n \geq j \geq 1} [(\neg c_j \wedge d_j) \wedge \bigwedge_{1 \leq i \leq j-1} ((c_i \wedge d_i) \vee (\neg c_i \wedge \neg d_i)) \wedge \bigwedge_{j+1 \leq i \leq n} (c_i \wedge \neg d_i)]$ as a disjunction of formulae starting from $j = n$ to $j = 1$

(the disjunction is for j where first flip occurs starting from n to 1, in my answer - $d_n \wedge \neg c_n$ in first and $d_{n-1} \wedge \neg c_{n-1}$ in second line).

I also correctly wrote the conjunction (XNOR) to say c and d values are same from $j-1$ to 1,

$\bigwedge_{n-1 \geq i \geq 1} ((c_i \wedge d_i) \vee (\neg c_i \wedge \neg d_i))$ in the first line and

$\bigwedge_{n-2 \leq i \leq 1} ((c_i \wedge d_i) \vee (\neg c_i \wedge \neg d_i))$ in the second line. (in expanded form)

I also wrote the conjunction to represent the flipped bits, $\neg d_n \wedge c_n$ in the second line and similarly for the last one.

(However, due to time constraints in the last line, I couldn't mention $d_1 \vee \neg c_1$ at the end but it is clear from above - we shift $d_i \wedge \neg c_i$ towards end, I sincerely apologise.)

I feel I have mentioned everything in accordance with the rubric (the three points - Disj, Conj_same, Conj_flip as well as the expanded formula is same with indices from n to 1), I humbly request you to regrade my answer as I should get more marks.

Thanks and best regards,

Fixed. Your answer was unclear and I couldn't understand the meaning of the expression that was written

Reviewed on: Oct 02

Question 4

Q2 (b) (i)

2 / 2 pts

✓ + 0.5 pts $\mathcal{C} = \{0\}$

✓ + 1 pt $\mathcal{F} = \{*/2\}$ (it is ok if it is sq/1 where $\text{sq}(x) = x * x$)

✓ + 0.5 pts $\mathcal{P} = \{</2\}$ or any other relation that can be used instead of $<$

+ 0 pts Incorrect

Question 5

Q2 (b) (ii)

4 / 4 pts

+ 0 pts Incorrect

$$\alpha = \forall x. \forall y. [x < y \supset \exists z. [x < z \wedge z < y]]$$

✓ + 0.5 pts $\forall x \forall y$

✓ + 1 pt $x < y$

✓ + 0.5 pts $\exists z. [x < z \wedge z < y]$

+ 0 pts Incorrect

$$\beta = \forall x. [0 < x \supset \exists y. [\exists z. [x = y * y \wedge x = z * z \wedge 0 < y \wedge z < 0]]]$$

✓ + 0.5 pts Three variables, $\forall x, \exists y, \exists z$

✓ + 0.5 pts $0 < x$ (use the same symbol as in the relation set)

✓ + 0.5 pts $x = y * y \wedge x = z * z$

✓ + 0.5 pts $0 < y$ and $z < 0$

+ 0 pts Incorrect

Question 6

Q3 (a)

4 / 4 pts

✓ + 0.5 pts $(p \wedge s) \supset (r \vee s) \Leftrightarrow \neg(p \wedge s) \vee (r \vee s)$ and $(r \vee s) \supset (p \wedge s) \Leftrightarrow \neg(r \vee s) \vee (p \wedge s)$

✓ + 0.5 pts $\neg(p \wedge s) \vee (r \vee s) \Leftrightarrow (\neg p \vee \neg s) \vee (r \vee s)$ and $\neg(r \vee s) \vee (p \wedge s) \Leftrightarrow (\neg r \wedge \neg s) \vee (p \wedge s)$

✓ + 0.5 pts $(\neg p \vee \neg s) \vee (r \vee s) \Leftrightarrow (\neg p \vee r \vee T)$

✓ + 0.5 pts $(\neg p \vee r \vee T) \Leftrightarrow T$

✓ + 0.5 pts $(\neg r \wedge \neg s) \vee (p \wedge s) \Leftrightarrow (\neg r \vee (p \wedge s)) \wedge (\neg s \vee (p \wedge s))$

✓ + 0.5 pts $(\neg r \vee (p \wedge s)) \wedge (\neg s \vee (p \wedge s)) \Leftrightarrow (\neg r \vee p) \wedge (\neg r \vee s) \wedge (\neg s \vee p) \wedge (\neg s \vee s)$

✓ + 0.5 pts $(\neg r \vee p) \wedge (\neg r \vee s) \wedge (\neg s \vee p) \wedge (\neg s \vee s) \Leftrightarrow (\neg r \vee p) \wedge (\neg r \vee s) \wedge (\neg s \vee p) \wedge T$

✓ + 0.5 pts $T \wedge ((\neg r \vee p) \wedge (\neg r \vee s) \wedge (\neg s \vee p) \wedge T) \Leftrightarrow (\neg r \vee p) \wedge (\neg r \vee s) \wedge (\neg s \vee p)$

+ 0 pts Incorrect/Not attempted

Did not clean the expressions containing s and ~s

Question 7

Q3 (b)

6 / 6 pts

✓ + 1 pt CNF expression to consider:
 $\varphi = \{\{\neg r, p\}, \{\neg r, s\}, \{\neg s, p\}, \{r \vee s\}, \{\neg s\}\}$

✓ + 1 pt Clean this expression since $\{\neg s\} \subseteq \{\neg s, p\}$. Get
 $\varphi^* = \{\{\neg r, p\}, \{\neg r, s\}, \{r \vee s\}, \{\neg s\}\}$

✓ + 1.5 pts Resolve using r . ($\{s\} \cup \{s\} = \{s\}$, and $\neg s$ stays untouched.
 $\text{resolve}(\varphi^*, r) = \{\{p, s\}, \{s\}, \{\neg s\}\}$

✓ + 1 pt Clean this expression since $\{s\} \subseteq \{p, s\}$. Get
 $\varphi_1^* = \{\{s\}, \{\neg s\}\}$

✓ + 1.5 pts Resolve using s .
 $\text{resolve}(\varphi_1^*, s) = \{\emptyset\}$ so the logical consequence holds

+ 0 pts Incorrect/Not attempted

Question 9

Q4 (b)

Resolved 2 / 4 pts

+ 0 pts Incorrect

 \Rightarrow direction: Suppose ϕ_{sat} is valid.+ 0.5 pts For any τ , $\tau \models \bigvee \{\phi'_\tau \mid \tau' \text{ a valuation over } \text{atoms}(\phi)\}$ + 1 pt $\tau \models \phi'_\tau$ for some τ' (by the satisfaction of disjunction)+ 0.5 pts There is some τ_0 such that $\tau_0 \models \phi$ (by the induction statement for (a)) \Leftarrow direction: Suppose ϕ is satisfiable.✓ + 1 pt There is some τ such that $\tau \models \phi$, iff $\models \phi_\tau$ (by (a))✓ + 1 pt If $\models \phi_\tau$ then $\models \phi_\tau \vee \psi$ for any ψ , and $\phi_{\text{sat}} = \phi_\tau \vee \phi'$ (where $\phi' = \bigvee_{\tau' \neq \tau} \{\phi'_\tau \mid \tau' \text{ a valuation over } \text{atoms}(\phi)\}$)

🔄 Regrade Request

Submitted on: Oct 01

Dear sir/ma'am,

For the \Rightarrow direction,

I mentioned that if ϕ_{sat} is valid, then there would exist one τ' such that $\phi_{\tau'}$ is valid by part a. (this is true as every $\phi_{\tau'}$ for some τ' is either a validity or unsat based on our construction and we take the disjunction.)

Then I concluded by the part a statement, as $\phi_{\tau'}$ is valid, $\tau' \models \phi$ and hence ϕ is satisfiable. So, I humbly request you to please regrade as I feel I it is correct and I deserve more marks for the \Rightarrow direction as per the three/last 2 rubric points.

(I apologise for the mistake I did in part a - my construction replaced the positive literals in τ by validity $\alpha \supset \phi$ but I forgot to mention that we replace the negative literals by negation of the validity - however the proof for \Rightarrow direction in b still holds.)

Thanks and best regards,

Just because a disjunction is valid does not imply that a single disjunct is valid, merely that each valuation satisfies some disjunct. No points.

Reviewed on: Oct 02

Question 10

Q5

10 / 10 pts

✓ + 0.5 pts Apply DT to $(p \supset q) \supset (p \supset r), \neg q \supset \neg p \vdash \neg r \supset \neg p$ to get $(p \supset q) \supset (p \supset r) \vdash (\neg q \supset \neg p) \supset (\neg r \supset \neg p)$

✓ + 0.5 pts Get $\neg r \supset \neg p$ by applying MP to $(p \supset r) \supset (\neg r \supset \neg p)$ (still to be proved) and $p \supset r$ (also to be proved)

Show that $\vdash (p \supset r) \supset (\neg r \supset \neg p)$

✓ + 1 pt Use MP on $(\neg p \supset r) \supset \neg p$ and $\neg p \supset r$ (still needs a proof) and DT to get the result

✓ + 1.5 pts Use MP on $(\neg p \supset \neg r) \supset (\neg p \supset r) \supset \neg p$ (obtained by H3) and $(\neg p \supset \neg r)$ (obtained by Ax + DT) to get $(\neg p \supset r) \supset \neg p$

Show that $p \supset r \vdash \neg p \supset r$

✓ + 0.5 pts Apply DT to $p \supset r, \neg\neg p \vdash r$ to get the result

Get r by MP on $p \supset r$ (obtained by Ax) and p

✓ + 1 pt Get p by MP on $(\neg p \supset \neg p) \supset p$ and $\neg p \supset \neg p$ (proved by Ax + DT)

✓ + 1.5 pts Get $(\neg p \supset \neg p) \supset p$ by MP on $(\neg p \supset p) \supset (\neg p \supset \neg p) \supset p$ (obtained by H3) and $\neg p \supset \neg p$ (obtained by Ax + DT)

✓ + 0.5 pts Use MP with $(p \supset q) \supset (p \supset r)$ and $p \supset q$ to get $p \supset r$ (Still have to produce a proof of $p \supset q$)

✓ + 0.5 pts Get $(p \supset q) \supset (p \supset r), \neg q \supset \neg p, \neg r \vdash \neg r$ by Ax

Show that $\neg q \supset \neg p \vdash p \supset q$

✓ + 1 pt Get $\neg q \supset \neg p \vdash p \supset q$ by DT on $\neg q \supset \neg p, p \vdash q$

Obtain $\neg q \supset \neg p, p \vdash q$ by MP on $(\neg q \supset p) \supset q$ and $\neg q \supset p$ (by Ax + DT)

✓ + 1.5 pts Obtain $(\neg q \supset \neg p) \supset q$ by MP on $(\neg q \supset \neg p) \supset (\neg q \supset p) \supset q$ (obtained by H3) and $\neg q \supset \neg p$ (obtained by Ax)

+ 0 pts Incorrect

Name: KUSNAGRA

GUPTA

Entry Number:

2021CS50592

1

Indian Institute of Technology Delhi

COL703: Logic for Computer Science

MID-TERM EXAM

DATE: Friday the 13th of September 2024

DURATION: 2 hours

MAXIMUM MARKS: 50

Q1 (10)	Q2 (10)	Q3 (10)	Q4 (10)	Q5 (10)	Total (50)

Instructions: Write your name and entry number at the top of each sheet. Answer all questions only in the boxes provided. Solutions outside the assigned box will not be graded. Make reasonable assumptions and state them wherever necessary.

Attestation: I agree to abide by the Honour Code of IIT Delhi.

Signature:

Kushagra

Q1. (10 marks) The length of an expression is often not a very good measure of how complex it is. To this end, we define new notions for propositional and first-order expressions.

(a) (5 marks) For propositional expressions, use the number of distinct propositional atoms, denoted by atn . For example,

$$atn(p) = 1$$

$$atn(p \wedge (q \vee p)) = 2$$

$$atn(p \vee (\neg p \wedge q)) = 2$$

$$atn(p \wedge (\neg(p \supset r))) = 2$$

Define atn inductively for expressions generated by the following grammar.

$$\alpha, \beta := p \mid \perp \mid \neg\alpha \mid \alpha \wedge \beta \mid \alpha \vee \beta \mid \alpha \supset \beta \quad \text{where } p \in AP$$

~~$atn(p) = 1$~~ ~~$atn(\perp) = 0$~~ ~~$atn(\neg\alpha) = atn(\alpha)$~~

We also define ats inductively in order to define atn :

$$ats(p) = \{p\}, \quad ats(\perp) = \emptyset, \quad ats(\neg\alpha) = ats(\alpha)$$

$$ats(\alpha \wedge \beta) = ats(\alpha) \cup ats(\beta) \quad ats(\alpha \vee \beta) = ats(\alpha) \cup ats(\beta)$$

$$ats(\alpha \supset \beta) = ats(\alpha) \cup ats(\beta)$$

Now, $atn(p) = |ats(p)|$, $atn(\perp) = |ats(\perp)|$, $atn(\neg\alpha) = |ats(\neg\alpha)|$

$$atn(\alpha \wedge \beta) = |ats(\alpha \wedge \beta)|, \quad atn(\alpha \vee \beta) = |ats(\alpha \vee \beta)|, \quad atn(\alpha \supset \beta) = |ats(\alpha \supset \beta)|$$

(b) (5 marks) For first-order expressions, we use the maximum nesting depth of quantifiers, denoted by qd . For example,

$$qd(t_1 \equiv t_2) = 0$$

$$qd(\forall x. [x \equiv c]) = 1$$

$$qd(\exists x. [\exists y. [x \equiv y]] \wedge y \equiv c) = 2$$

$$qd(\exists x. [P(t_1) \wedge \forall y. [y \equiv c]]) = 2$$

Write an inductive definition for qd for first-order expressions generated by the following grammar.

$$\alpha, \beta := t_1 \equiv t_2 \mid P(t_1, \dots, t_n) \mid \neg\alpha \mid \alpha \wedge \beta \mid \alpha \vee \beta \mid \alpha \supset \beta \mid \exists x. [\alpha] \mid \forall x. [\alpha] \quad \text{where } P \text{ is an } n\text{-ary predicate symbol.}$$

$$qd(t_1 \equiv t_2) = 0 \quad qd(P(t_1 \dots t_n)) = 0$$

$$qd(\neg\alpha) = qd(\alpha) \quad qd(\alpha \wedge \beta) = \max(qd(\alpha), qd(\beta))$$

$$qd(\alpha \vee \beta) = \max(qd(\alpha), qd(\beta))$$

$$qd(\alpha \supset \beta) = \max(qd(\alpha), qd(\beta))$$

$$qd(\exists x [\alpha]) = qd(\alpha) + 1, \quad qd(\forall x [\alpha]) = qd(\alpha) + 1$$

Q2. (10 marks) Modelling in logics.

(a) (4 marks) Consider two n -bit binary numbers c_1, c_2, \dots, c_n and d_1, d_2, \dots, d_n . Let $AP = \{c_1, \dots, c_n, d_1, \dots, d_n\}$ be the set of propositional atoms. Any valuation τ sets c_i to T iff $c_i = 1$, and similarly for d_i . Write a propositional expression for $d = c + 1$.

$$\begin{aligned} & (d_n \wedge \neg c_n \wedge ((d_{n-1} \wedge c_{n-1}) \vee (\neg d_{n-1} \wedge \neg c_{n-1})) \wedge \dots \wedge (d_1 \wedge c_1) \vee (\neg d_1 \wedge \neg c_1)) \\ & \vee (\neg d_n \wedge c_n \wedge (d_{n-1} \wedge \neg c_{n-1}) \wedge ((d_{n-2} \wedge c_{n-2}) \vee (\neg d_{n-2} \wedge \neg c_{n-2})) \dots) \\ & \vee (\neg d_n \wedge c_n \wedge \neg d_{n-1} \wedge c_{n-1} \wedge \neg d_{n-2} \wedge c_{n-2} \wedge \dots \wedge \neg d_1 \wedge c_1) \end{aligned}$$

(b) i. (2 marks) Define a signature Σ required to express the following statements in first-order logic.

$$\begin{aligned} \mathcal{C} &= \{0\}, \quad \mathcal{F} = \{sq/1\} \\ \mathcal{P} &= \{L/2, LE/2\} \end{aligned}$$

ii. (4 marks) Express the following in FO_{Σ} .

• $[\alpha]$: Between any two real numbers, there is another real number.

$$\forall p [\forall q [\exists r [(LE(p, r) \wedge LE(r, q)) \vee (LE(q, r) \wedge LE(r, p))]]]$$

• $[\beta]$: Every positive real number has two real square roots, one positive and one negative.

$$(\forall p [L(0, p) \supset (\exists r [L(0, r) \wedge (sq(r) \equiv p)])]) \wedge (\forall p [L(0, p) \supset (\exists r [L(r, 0) \wedge (sq(r) \equiv p)])])$$

Q3. (10 marks) CNF and Resolution.

(a) (4 marks) Convert $((p \wedge s) \supset (r \vee s)) \wedge ((r \vee s) \supset (p \wedge s))$ to an equivalent CNF expression. Justify each step clearly.

$$\begin{aligned} (p \wedge s) \supset (r \vee s) & \equiv \neg(p \wedge s) \vee (r \vee s) \equiv (\neg p \vee \neg s \vee r \vee s) \quad ① \\ (r \vee s) \supset (p \wedge s) & \equiv \neg(r \vee s) \vee (p \wedge s) \equiv (\neg r \wedge \neg s) \vee (p \wedge s) \quad ② \\ \text{By distributivity of } \wedge \text{ over } \vee. & \equiv (\neg r \vee p) \wedge (\neg r \vee s) \wedge (\neg s \vee p) \wedge (\neg s \vee s) \\ & \equiv (\neg r \vee p) \wedge (\neg r \vee s) \wedge (\neg s \vee p) \wedge (\neg s \vee s) \\ & \equiv ((\neg r \vee p) \wedge (\neg r \vee s) \wedge (\neg s \vee p) \wedge (\neg s \vee s)) \end{aligned}$$

$$① \text{ \& } ② \text{ followed by identity } a \supset b \equiv \neg a \vee b \quad \& \quad \neg(a \wedge b) \equiv \neg a \vee \neg b$$

$$\begin{aligned} \text{So } ((p \wedge s) \supset (r \vee s)) \wedge ((r \vee s) \supset (p \wedge s)) & \\ \equiv ((\neg p \vee \neg s \vee r \vee s) \wedge (\neg r \vee p) \wedge (\neg r \vee s) \wedge (\neg s \vee p) \wedge (\neg s \vee s)) & \end{aligned}$$

$$\text{In CNF expression } \{\{p, s, r, s\}, \{r, p\}, \{r, s\}, \{s, p\}, \{s, s\}\}$$

(b) (6 marks) Use resolution to show that $\{(p \wedge s) \supset (r \vee s) \wedge ((r \vee s) \supset (p \wedge s)), r \vee s\} \models s$.

$\Gamma = \{(p \wedge s) \supset (r \vee s), (r \vee s) \supset (p \wedge s), r \vee s\}$
 First we convert each expression in Γ into CNF form
 $(\neg p \vee \neg s \vee r \vee s) \wedge ((\neg r \wedge \neg s) \vee (p \wedge s))$ as $a \supset b \equiv \neg a \vee b$
 $(\neg p \vee \neg s \vee r \vee s) \wedge (\neg r \vee p) \wedge (\neg r \vee s) \wedge (\neg s \vee p) \wedge (\neg s \vee s)$
 $\Delta = \{\{\neg p, \neg s, r, s\}, \{\neg r, p\}, \{\neg r, s\}, \{s, p\}, \{\neg s, s\}, \{r, s\}, \{s\}\}$
 First we clean Δ (added neg. of consequent for resol. refutation)
 $\Delta' = \{\{\neg r, p\}, \{\neg r, s\}, \{\neg s, p\}, \{r, s\}, \{s\}\}$ (as $\neg s \in \{s, p\}$)
 Now resolve with "p" = r, taking $\delta_1 = \{s, p\}$ & $\delta_2 = \{\neg r, s\}, \{\neg r, p\}$
 $\Delta'' = \{\{p, s\}, \{s\}, \{\neg s\}\}$
 Now, resolve with "p" = s, taking $\delta_1 = \{s\}, \{p, s\}$ & $\delta_2 = \{\neg s\}$
 $\Delta''' = \{\{p\}, \emptyset\}$
 Since Δ''' has \emptyset in set of clauses, it is UNSAT.
 $\therefore \Gamma \wedge \neg s$ is UNSAT or $\neg(\Gamma \supset s)$ is UNSAT
 $\therefore \Gamma \models s$ by resolution refutation

Q4. (10 marks) Encoding meta-logical concepts as PL expressions.

(a) (6 marks) For $\phi, \psi \in \text{PL}$, we say that ψ is an instance of ϕ , if one can simultaneously replace each atom p occurring in ϕ by some expression α_p , and obtain ψ . For any ϕ , and a valuation τ over atoms(ϕ), define an instance ϕ_τ of ϕ such that ϕ_τ is valid iff $\tau \models \phi$.

Given valuation τ , construct $\alpha = \bigwedge_{p_i \in \tau} p_i \wedge \bigwedge_{p_j \notin \tau} \neg p_j$ (if $\tau = 0$, $\tau: p=0, q=1$, $p \notin \tau, q \in \tau$)
 Consider $\phi \wedge \alpha$.
 Replace each atom in ϕ by $\phi \wedge \alpha$ to get ϕ_τ ($\phi \wedge \alpha$ is $\phi \supset \alpha \wedge \alpha \supset \phi$)
 It is easy to see why it is valid iff $\tau \models \phi$.

(b) (4 marks) Let $\phi_{\text{sat}} = \bigvee \{\phi_\tau \mid \tau \text{ a valuation over atoms}(\phi)\}$. Show that ϕ_{sat} is valid iff ϕ is satisfiable.

\Leftarrow If ϕ is satisfiable \exists a valuation τ' s.t. $\tau' \models \phi$
 $\Rightarrow \phi_{\tau'}$ is valid (by part a)
 Since ϕ_{sat} is disjunction of ϕ_τ $\Rightarrow \phi_{\text{sat}}$ is valid.
 \Rightarrow If ϕ_{sat} is valid, \exists some τ' such that $\phi_{\tau'}$ is valid.
 \therefore by part a, $\tau' \models \phi$
 So ϕ is satisfiable
 Pure Bk do's good

[illegible]